LeanSAT.lean
@@ -1,5 +1,4 @@
 import LeanSAT.AuxDefs
 import LeanSAT.CNF
-import LeanSAT.Constraint
-import LeanSAT.EncCNF
+import LeanSAT.Encode
 import LeanSAT.Solver
