LeanSAT/Encode.lean
@@ -1,0 +1,2 @@
+import LeanSAT.Encode.EncCNF
+import LeanSAT.Encode.Card
